

# Assignment W3

Enoch Lau

September 21, 2025

## 1 Q1.

(a)  $\overline{D} \cup E = \{1, 2, 4, 5, 6, 7, 8, 9, 10\}$

(b)  $C \cup (D \cap E) = \{2, 3, 5, 7, 8, 9, 10\}$

(c)  $\overline{(C \cap E)} = \{1, 3, 4, 5, 6, 7, 8, 10\}$

(d)  $(C \cup E) - D = \{1, 2, 7\}$

## 2 Q2.

Problem: For all integers  $x, y$ , and  $z$ , if  $7x^2 - 3y - z + 5xy + y^2z$  is odd, then  $y$  is odd or  $(x - z)$  is odd.

This will be a proof by contrapositive. We will prove that if  $y$  is even and  $(x - z)$  is even, then  $7x^2 - 3y - z + 5xy + y^2z$  is even.

Notice that if  $(x - z)$  is even, then either both  $x$  and  $z$  are even, or both are odd. Proof:

$$2a - 2b = 2(a - b), \text{ even}$$

$$(2a + 1) - (2b + 1) = 2(a - b), \text{ even}$$

$$(2a + 1) - 2b = 2(a - b) + 1, \text{ odd}$$

$$2a - 2b + 1 = 2(a - b) + 1, \text{ odd}$$

Note that  $(a - b)$  is an integer because both  $a$  and  $b$  are integers.

Assumption:  $2 \mid y$  and  $2 \mid (x - z)$

Case 1: Given  $x, y, z \in \mathbb{Z}$ , and they are all even. Let  $a, b, c \in \mathbb{Z} : x = 2a, y = 2b, z = 2c$

$$\begin{aligned} & 7(2a)^2 - 3(2b) - 2c + 5(2a)(2b) + (2b)^2(2c) \\ &= 28a^2 - 6b - 2c + 20ab + 8b^2c \\ &= 2(14a^2 - 3b - c + 10ab + 4b^2c) \end{aligned}$$

$\therefore a, b, c \in \mathbb{Z}$ , the expression inside the parenthesis is an integer,

$\therefore$  For  $x, y, z$  being even, the expression is even.

Case 2: Given  $x, y, z \in \mathbb{Z}$ , and both  $x$  and  $z$  are odd,  $y$  being even. Let  $a, b, c \in \mathbb{Z} : x = 2a + 1, y = 2b, z = 2c + 1$

$$\begin{aligned} & 7(2a + 1)^2 - 3(2b) - (2c + 1) + 5(2a + 1)(2b) + (2b)^2(2c + 1) \\ &= 7(4a^2 + 4a + 1) - 6b - 2c - 1 + (10a + 5)(2b) + (4b^2)(2c + 1) \\ &= 28a^2 + 14a + 7 - 6b - 2c - 1 + 20ab + 10b + 8b^2c + 4b^2 \\ &= 28a^2 + 14a + 6 - 6b - 2c + 20ab + 10b + 8b^2c + 4b^2 \\ &= 2(14a^2 + 7a + 3 - 3b - c + 10ab + 5b + 4b^2c + 2b^2) \end{aligned}$$

$\therefore a, b, c \in \mathbb{Z}$ , the expression inside the parenthesis is an integer,

$\therefore$  For  $y$  being even,  $x, z$  being odd, the expression is even.

The expression is even for both cases, so we have proved the contrapositive.  $\square$

### 3 Q3.

Problem: For all integers  $r, s$ , if  $14|(r + s)$  and  $21|r^3$  then  $7|(3r^2(r - 5) + 15s^2)$

Assuming  $14|(r + s)$  and  $21|r^3$ , and  $r, s \in \mathbb{Z}$ .

By Transitivity of Divisibility,  $7|(r + s)$  and  $7|r^3$ , because  $7|14$  and  $7|21$ .

By Divisibility of Integer Combinations,  $7|3r^3 - 15(r - s)(r + s)$ , because  $3, (-15)(r - s) \in \mathbb{Z}$ .

$$\begin{aligned} 3r^3 - 15(r - s)(r + s) &= 3r^3 - 15(r^2 - s^2) \\ &= 3r^3 - 15r^2 + 15s^2 \\ &= 3r^2(r - 5) + 15s^2 \end{aligned}$$

Thus,  $7|(3r^2(r - 5) + 15s^2)$ , as required. □

## 4 Q4.

Problem:  $\forall x \in \mathbb{Z}, [(2x \neq 6) \implies (\forall z \in \mathbb{Z}, \exists y \in \mathbb{Z}, x - 7 \neq (z - y + 5)(z^2 + 1) - 4)]$

Proof: Assume that  $2x \neq 6$ . Notice that  $2x \neq 6 \iff x \neq 3$ .

Now, choose  $y = z + 5$  for any  $z \in \mathbb{Z}$ . Clearly,  $z + 5$  is an integer.

Substituting back:

$$\begin{aligned}(z - y + 5)(z^2 + 1) - 4 &= (z - (z + 5) + 5)(z^2 + 1) - 4 \\ &= (0)(z^2 + 1) - 4 = -4\end{aligned}$$

Therefore:  $x - 7 \neq -4$ , and

$$x - 7 \neq -4 \iff x \neq 3$$

Since we assumed  $x \neq 3$  in our hypothesis, this always holds.

Thus, for any  $x \neq 3$  and any  $z \in \mathbb{Z}$ , we can choose  $y = z + 5$  to ensure that  $x - 7 \neq (z - y + 5)(z^2 + 1) - 4$ .

□

## 5 Q5.

(a) This is false. Consider the number 2. It is not in  $F$ , because  $4 \cdot \frac{1}{2} = 2$  and  $\frac{1}{2} \notin \mathbb{Z}$ , and also not in  $G$ , because  $3 \nmid (2 - 1)$ . Therefore  $F \cup G$  does not contain 2, and so  $\overline{F \cup G}$  contains 2, which means  $\overline{F \cup G} \neq \emptyset$ .

(b) This is true.  $\forall x \in \mathbb{Z}$ , if  $x \in H$ , then  $24 \mid (x + 8)$ , and by definition,  $\exists k \in \mathbb{Z}, x + 8 = 24k$ .

So  $x + 8 = 24k$

$$x = 24k - 8$$

$$x = 4(6k - 2)$$

So there exists an integer,  $(6k - 2)$ , such that  $x = 4(6k - 2)$ , hence  $4 \mid x$ , from which follows  $x \in F$ .

And also from  $x + 8 = 24k$ ,

$$x - 1 = 24k - 9$$

$$x - 1 = 3(8k - 3)$$

So there exists an integer,  $(8k - 3)$ , such that  $x - 1 = 3(8k - 3)$ , hence  $3 \mid (x - 1)$ , from which follows  $x \in G$ .

Therefore, if  $x \in H$ , then  $x \in F$  and  $x \in G$ , so  $x \in F \cap G$ .  $\square$

## 6 Q6.

- (a)  $S = K, P = P_3$
- (b)  $S = J, P = P_4$
- (c)  $S = L, P = P_1$
- (d)  $S = M, P = P_2$